lib/utils.v
@@ -1912,3 +1912,22 @@ Definition interchange op1 op2 :=
 End SopSisS.
 
 End OperationProperties.
+
+Ltac match_inv :=
+  repeat match goal with
+  | H : bind (fun x : _ => _) _ = Some _ |- _ =>
+    apply bind_inv in H;
+    let x := fresh x in
+    let E := fresh "E" in
+    destruct H as (x & H & E);
+    simpl in H; simpl in E
+  | H : (if ?b then _ else _) = Some _ |- _ =>
+    let E := fresh "E" in
+    destruct b eqn:E;
+    try discriminate
+  | H : match ?E with _ => _ end = _ |- _ =>
+    destruct E eqn:?; try discriminate
+  | H : Some _ = Some _ |- _ => inv H
+  | H : ?O = Some _ |- context[bind _ ?O] => rewrite H; simpl
+  | H : True |- _ => clear H
+  end.
